n-message receivefrom_nodup

theories/aneris_lang/lib/nodup.v
@@ -1,5 +1,5 @@
 From aneris.aneris_lang Require Import proofmode notation.
-From aneris.aneris_lang.lib Require Import util set network_util.
+From aneris.aneris_lang.lib Require Import util set list network_util.
 From iris_string_ident Require Import ltac2_string_ident.
 Set Default Proof Using "Type".
 Import Network.
@@ -10,6 +10,17 @@ Definition receivefrom_nodup : val :=
      let: "msg" := unSOME (ReceiveFrom "socket") in
      if: set_mem "msg" "msgs" then "loop" #()
      else ("msg", set_add "msg" "msgs")) #().
+
+Definition receivefrom_nodup_n : val :=
+  rec: "receivefrom_nodup_n" "socket" "msgs" "n" :=
+    if: "n" = #0 then (list_nil, "msgs") else
+    let: "tmp" := receivefrom_nodup "socket" "msgs" in
+    let: "m" := Fst "tmp" in
+    let: "msgs'" := Snd "tmp" in
+    let: "tailmsgs" := "receivefrom_nodup_n" "socket" "msgs'" ("n" - #1) in
+    let: "ms" := Fst "tailmsgs" in
+    let: "msgs''" := Snd "tailmsgs" in
+    ("m" :: "ms", "msgs''").
 
 Definition nodup_init : val := set_empty.
 
@@ -44,7 +55,8 @@ Section nodup_specs.
     {{{ h ↪[ip] s ∗ a ⤇ φ ∗ a ⤳ (R, T) ∗ ⌜is_nodup R a v⌝ }}}
       receivefrom_nodup #(LitSocket h) v @[ip]
     {{{ m v', RET ((#(m_body m), #(m_sender m)), v')%V;
-          h ↪[ip] s ∗ a ⤳ ({[m]} ∪ R, T) ∗ ⌜is_nodup ({[m]} ∪ R) a v'⌝ ∗ φ m }}}.
+          h ↪[ip] s ∗ a ⤳ ({[m]} ∪ R, T) ∗ φ m ∗
+          ⌜is_nodup ({[m]} ∪ R) a v'⌝ ∗ ⌜m ∉ R⌝ }}}.
   Proof.
     iIntros (-> ?? Φ) "(Hh & #Hφ & Ha & [%Hv %Hdest]) HΦ".
     wp_rec. do 3 wp_pure _.
@@ -67,7 +79,7 @@ Section nodup_specs.
       wp_pures. iApply "HΦ".
       iFrame. iPureIntro.
       rewrite -(gset_map_singleton (λ m, (m_body m, m_sender m)) m) -gset_map_union in Hv'.
-      split; auto.
+      do 2 (split; auto).
       intros ? [-> %elem_of_singleton_1 | ?]%elem_of_union; [done|].
       by apply Hdest.
     - wp_apply wp_unSOME; [done|]; iIntros "_".
@@ -77,6 +89,34 @@ Section nodup_specs.
       { by apply (gset_map_correct1 (λ m, (m_body m, m_sender m))) in Hm. }
       wp_if.
       iApply ("IH" with "[//] [//] Hh Ha HΦ").
+  Qed.
+
+  Lemma wp_receivefrom_nodup_n ip a φ h s R T v (n : nat) :
+    ip = ip_of_address a →
+    saddress s = Some a →
+    sblock s = true →
+    {{{ h ↪[ip] s ∗ a ⤇ φ ∗ a ⤳ (R, T) ∗ ⌜is_nodup R a v⌝ }}}
+      receivefrom_nodup_n #(LitSocket h) v #n @[ip]
+    {{{ ms vms v' R', RET (vms, v')%V;
+          ⌜is_nodup R' a v'⌝ ∗ ⌜length ms = n⌝ ∗
+          ⌜is_list (map (λ m, (#(m_body m), #(m_sender m))%V) ms) vms⌝ ∗
+          h ↪[ip] s ∗ a ⤳ (R', T) ∗ [∗ list] m ∈ ms, φ m }}}.
+  Proof.
+    iIntros (-> ?? Φ) "(Hh & #Hφ & Ha & %Hv) HΦ".
+    iInduction n as [|n'] "IH" forall (Φ v R Hv); wp_rec; wp_pures.
+    { iApply ("HΦ" $! []). iFrame. auto. }
+    wp_apply (wp_receivefrom_nodup with "[$Hh $Hφ $Ha //]"); [done..|].
+    iIntros (m v') "(Hh & Ha & Hm & %Hv' & %Hin)".
+    wp_pures.
+    assert ((S n' - 1)%Z = n') as -> by lia.
+    wp_apply ("IH" with "[//] Hh Ha").
+    iIntros (ms vms v'' R') "(%Hv'' & %Hlen & %Hvms & Hh & Ha & Hφms)".
+    wp_pures.
+    wp_apply wp_list_cons; [done|].
+    iIntros (vms' Hvms'). wp_pures.
+    iApply ("HΦ" $! (m :: ms)).
+    iFrame. iFrame "%".
+    simpl. rewrite Hlen //.
   Qed.
 
 End nodup_specs.
